\begin{dmath*}
piss = 1
\end{dmath*}
\begin{dmath*}
Pss = 1
\end{dmath*}
\begin{dmath*}
ZAss = 1
\end{dmath*}
\begin{dmath*}
ZMss = 1
\end{dmath*}
\begin{dmath*}
Rss = \frac{1}{{{\beta}}}-1
\end{dmath*}
\begin{dmath*}
LAMBss = \frac{{Pss}\, \left({{\psi}}-1\right)}{{{\psi}}}
\end{dmath*}
\begin{dmath*}
Wss = {LAMBss}\, {ZAss}
\end{dmath*}
\begin{dmath*}
Yss = \left(\frac{{Wss}}{{Pss}\, {{\varphi}}}\right)^{\frac{1}{{{\phi}}+{{\sigma}}}}
\end{dmath*}
\begin{dmath*}
Lss = {Yss}
\end{dmath*}
\begin{dmath*}
Css = {Yss}
\end{dmath*}
% Equation 1
\begin{dmath}
{{\hat{\pi}}}_{t}={{\hat{P}}}_{t}-{{\hat{P}}}_{t-1}
\end{dmath}
% Equation 2
\begin{dmath}
{{\hat{\pi}}}_{t}={{\beta}}\, {{\hat{\pi}}}_{t+1}+\frac{{{\hat{\lambda}}}_{t}\, \left(1-{{\theta}}\right)\, \left(1-{{\beta}}\, {{\theta}}\right)}{{{\theta}}}
\end{dmath}
% Equation 3
\begin{dmath}
{{\varphi}}\, {{\hat{L}}}_{t}+{{\sigma}}\, {{\hat{Y}}}_{t}={{\hat{W}}}_{t}-{{\hat{P}}}_{t}
\end{dmath}
% Equation 4
\begin{dmath}
{{\hat{Y}}}_{t}={{\hat{Y}}}_{t+1}-\frac{{{\beta}}}{{{\sigma}}}\, \left({{\hat{R}}}_{t}-{{\hat{\pi}}}_{t+1}\right)
\end{dmath}
% Equation 5
\begin{dmath}
{{\hat{\lambda}}}_{t}={{\hat{W}}}_{t}-{{\hat{Z}^A}}_{t}-{{\hat{P}}}_{t}
\end{dmath}
% Equation 6
\begin{dmath}
{{\hat{Y}}}_{t}={{\hat{L}}}_{t}+{{\hat{Z}^A}}_{t}
\end{dmath}
% Equation 7
\begin{dmath}
{{\hat{R}}}_{t}={{\gamma_R}}\, {{\hat{R}}}_{t-1}+\left(1-{{\gamma_R}}\right)\, \left({{\hat{\pi}}}_{t}\, {{\gamma_\pi}}+{{\hat{Y}}}_{t}\, {{\gamma_Y}}\right)+{{\hat{Z}^M}}_{t}
\end{dmath}
% Equation 8
\begin{dmath}
{{\hat{Z}^A}}_{t}={{\rho_A}}\, {{\hat{Z}^A}}_{t-1}+{{\varepsilon_A}}_{t}
\end{dmath}
% Equation 9
\begin{dmath}
{{\hat{Z}^M}}_{t}={{\rho_M}}\, {{\hat{Z}^M}}_{t-1}+{{\varepsilon_M}}_{t}
\end{dmath}
