\begin{dmath*}
piss = 1
\end{dmath*}
\begin{dmath*}
Pss = 1
\end{dmath*}
\begin{dmath*}
ZAss = 1
\end{dmath*}
\begin{dmath*}
ZMss = 1
\end{dmath*}
\begin{dmath*}
Rss = \frac{1}{{{\beta}}}-1
\end{dmath*}
\begin{dmath*}
LAMBss = \frac{{{\psi}}-1}{{{\psi}}}
\end{dmath*}
\begin{dmath*}
Wss = \frac{{{\psi}}-1}{{{\psi}}}
\end{dmath*}
\begin{dmath*}
Yss = \left(\frac{\frac{{{\psi}}-1}{{{\psi}}}}{{{\varphi}}}\right)^{\frac{1}{{{\phi}}+{{\sigma}}}}
\end{dmath*}
\begin{dmath*}
Lss = \left(\frac{\frac{{{\psi}}-1}{{{\psi}}}}{{{\varphi}}}\right)^{\frac{1}{{{\phi}}+{{\sigma}}}}
\end{dmath*}
\begin{dmath*}
Css = \left(\frac{\frac{{{\psi}}-1}{{{\psi}}}}{{{\varphi}}}\right)^{\frac{1}{{{\phi}}+{{\sigma}}}}
\end{dmath*}
% Equation 1
\begin{dmath}
{{\hat{\pi}}}=0
\end{dmath}
% Equation 2
\begin{dmath}
{{\hat{\pi}}}={{\beta}}\, {{\hat{\pi}}}+\frac{{{\hat{\lambda}}}\, \left(1-{{\theta}}\right)\, \left(1-{{\beta}}\, {{\theta}}\right)}{{{\theta}}}
\end{dmath}
% Equation 3
\begin{dmath}
{{\varphi}}\, {{\hat{L}}}+{{\sigma}}\, {{\hat{Y}}}={{\hat{W}}}-{{\hat{P}}}
\end{dmath}
% Equation 4
\begin{dmath}
{{\hat{Y}}}={{\hat{Y}}}-\frac{{{\beta}}}{{{\sigma}}}\, \left({{\hat{R}}}-{{\hat{\pi}}}\right)
\end{dmath}
% Equation 5
\begin{dmath}
{{\hat{\lambda}}}={{\hat{W}}}-{{\hat{Z}^A}}-{{\hat{P}}}
\end{dmath}
% Equation 6
\begin{dmath}
{{\hat{Y}}}={{\hat{L}}}+{{\hat{Z}^A}}
\end{dmath}
% Equation 7
\begin{dmath}
{{\hat{R}}}={{\hat{R}}}\, {{\gamma_R}}+\left(1-{{\gamma_R}}\right)\, \left({{\hat{\pi}}}\, {{\gamma_\pi}}+{{\hat{Y}}}\, {{\gamma_Y}}\right)+{{\hat{Z}^M}}
\end{dmath}
% Equation 8
\begin{dmath}
{{\hat{Z}^A}}={{\hat{Z}^A}}\, {{\rho_A}}+{{\varepsilon_A}}
\end{dmath}
% Equation 9
\begin{dmath}
{{\hat{Z}^M}}={{\hat{Z}^M}}\, {{\rho_M}}+{{\varepsilon_M}}
\end{dmath}
