\begin{dmath*}
thetaP = 0.7
\end{dmath*}
\begin{dmath*}
thetaZ = 0.7
\end{dmath*}
\begin{dmath*}
P1ss = 1
\end{dmath*}
\begin{dmath*}
P2ss = 0.7
\end{dmath*}
\begin{dmath*}
ZA1ss = 1
\end{dmath*}
\begin{dmath*}
ZA2ss = 0.7
\end{dmath*}
\begin{dmath*}
ZMss = 1
\end{dmath*}
\begin{dmath*}
piss = 1
\end{dmath*}
\begin{dmath*}
pi1ss = 1
\end{dmath*}
\begin{dmath*}
pi2ss = 1
\end{dmath*}
\begin{dmath*}
Rss = \frac{1}{{{\beta}}}-1
\end{dmath*}
\begin{dmath*}
Q1ss = \frac{{P1ss}\, {thetaP}^{1-{{\omega_{11}}}}}{{{\omega_{11}}}^{{{\omega_{11}}}}\, \left(1-{{\omega_{11}}}\right)^{1-{{\omega_{11}}}}}
\end{dmath*}
\begin{dmath*}
Q2ss = \frac{{P1ss}\, {thetaP}^{1-{{\omega_{11}}}}}{{{\omega_{21}}}^{{{\omega_{21}}}}\, \left(1-{{\omega_{21}}}\right)^{1-{{\omega_{21}}}}}
\end{dmath*}
\begin{dmath*}
LAMBDA1ss = \frac{{P1ss}\, \left({{\psi}}-1\right)}{{{\psi}}}
\end{dmath*}
\begin{dmath*}
LAMBDA2ss = \frac{\left({{\psi}}-1\right)\, {P2ss}}{{{\psi}}}
\end{dmath*}
\begin{dmath*}
W1ss = {ZA1ss}\, {LAMBDA1ss}
\end{dmath*}
\begin{dmath*}
W2ss = {LAMBDA2ss}\, {ZA2ss}
\end{dmath*}
\begin{dmath*}
a1ss = \left(\frac{{W1ss}\, {ZA1ss}^{{{\varphi}}}}{{{\phi}}\, {Q1ss}}\right)^{\frac{1}{{{\sigma}}}}
\end{dmath*}
\begin{dmath*}
a2ss = \left(\frac{{W2ss}\, {ZA2ss}^{{{\varphi}}}}{{{\phi}}\, {Q2ss}}\right)^{\frac{1}{{{\sigma}}}}
\end{dmath*}
\begin{dmath*}
Y1ss = \left(\frac{{Q1ss}\, {a1ss}}{{P1ss}}\right)^{\frac{{{\sigma}}}{{{\varphi}}+{{\sigma}}}}
\end{dmath*}
\begin{dmath*}
Y2ss = \left(\frac{{Q2ss}\, {a2ss}}{{P2ss}}\right)^{\frac{{{\sigma}}}{{{\varphi}}+{{\sigma}}}}
\end{dmath*}
\begin{dmath*}
C1ss = {a1ss}\, {Y1ss}^{\frac{\left(-{{\varphi}}\right)}{{{\sigma}}}}
\end{dmath*}
\begin{dmath*}
C2ss = {a2ss}\, {Y2ss}^{\frac{\left(-{{\varphi}}\right)}{{{\sigma}}}}
\end{dmath*}
\begin{dmath*}
C11ss = {C1ss}\, \left(\frac{{{\omega_{11}}}\, {P2ss}}{{P1ss}\, \left(1-{{\omega_{11}}}\right)}\right)^{1-{{\omega_{11}}}}
\end{dmath*}
\begin{dmath*}
C21ss = {C2ss}\, \left(\frac{{{\omega_{21}}}\, {P2ss}}{{P1ss}\, \left(1-{{\omega_{21}}}\right)}\right)^{1-{{\omega_{21}}}}
\end{dmath*}
\begin{dmath*}
C12ss = \frac{{P1ss}\, \left(1-{{\omega_{11}}}\right)\, {C11ss}}{{{\omega_{11}}}\, {P2ss}}
\end{dmath*}
\begin{dmath*}
C22ss = \frac{{P1ss}\, \left(1-{{\omega_{21}}}\right)\, {C21ss}}{{{\omega_{21}}}\, {P2ss}}
\end{dmath*}
\begin{dmath*}
L1ss = \frac{{Y1ss}}{{ZA1ss}}
\end{dmath*}
\begin{dmath*}
L2ss = \frac{{Y2ss}}{{ZA2ss}}
\end{dmath*}
\begin{dmath*}
Yss = {Y1ss}+{Y2ss}
\end{dmath*}
\begin{dmath*}
thetapi = \frac{{P1ss}\, {Y1ss}}{{P1ss}\, {Y1ss}+{P2ss}\, {Y2ss}}
\end{dmath*}
\begin{dmath*}
thetaY = \frac{{Y1ss}}{{Yss}}
\end{dmath*}
% Equation 1
\begin{dmath}
{{\hat{\pi}_{1}}}_{t}={{\hat{P}_{1}}}_{t}-{{\hat{P}_{1}}}_{t-1}
\end{dmath}
% Equation 2
\begin{dmath}
{{\hat{\pi}_{2}}}_{t}={{\hat{P}_{2}}}_{t}-{{\hat{P}_{2}}}_{t-1}
\end{dmath}
% Equation 3
\begin{dmath}
{{\hat{\pi}_{1}}}_{t}={{\beta}}\, {{\hat{\pi}_{x1}}}_{t}+\frac{{{\hat{\lambda}_{1}}}_{t}\, \left(1-{{\theta}}\right)\, \left(1-{{\beta}}\, {{\theta}}\right)}{{{\theta}}}
\end{dmath}
% Equation 4
\begin{dmath}
{{\hat{\pi}_{1}}}_{t}-{{\hat{\pi}_{x1}}}_{t-1}={{sunspot_{1}}}_{t}
\end{dmath}
% Equation 5
\begin{dmath}
{{\hat{\pi}_{2}}}_{t}={{\beta}}\, {{\hat{\pi}_{x2}}}_{t}+\frac{\left(1-{{\beta}}\, {{\theta}}\right)\, \left(1-{{\theta}}\right)\, {{\hat{\lambda}_{2}}}_{t}}{{{\theta}}}
\end{dmath}
% Equation 6
\begin{dmath}
{{\hat{\pi}_{2}}}_{t}-{{\hat{\pi}_{x2}}}_{t-1}={{sunspot_{2}}}_{t}
\end{dmath}
% Equation 7
\begin{dmath}
{{\hat{C}_{12}}}_{t}-{{\hat{C}_{11}}}_{t}={{\hat{P}_{1}}}_{t}-{{\hat{P}_{2}}}_{t}
\end{dmath}
% Equation 8
\begin{dmath}
{{\hat{C}_{22}}}_{t}-{{\hat{C}_{21}}}_{t}={{\hat{P}_{1}}}_{t}-{{\hat{P}_{2}}}_{t}
\end{dmath}
% Equation 9
\begin{dmath}
{{\hat{C}_{1}}}_{t}-{{\hat{C}_{11}}}_{t}=\left(1-{{\omega_{11}}}\right)\, \left({{\hat{P}_{1}}}_{t}-{{\hat{P}_{2}}}_{t}\right)
\end{dmath}
% Equation 10
\begin{dmath}
{{\hat{C}_{2}}}_{t}-{{\hat{C}_{21}}}_{t}=\left(1-{{\omega_{21}}}\right)\, \left({{\hat{P}_{1}}}_{t}-{{\hat{P}_{2}}}_{t}\right)
\end{dmath}
% Equation 11
\begin{dmath}
{{\hat{Q}_{1}}}_{t}={{\omega_{11}}}\, {{\hat{P}_{1}}}_{t}+\left(1-{{\omega_{11}}}\right)\, {{\hat{P}_{2}}}_{t}
\end{dmath}
% Equation 12
\begin{dmath}
{{\varphi}}\, {{\hat{L}_{1}}}_{t}+{{\sigma}}\, {{\hat{C}_{1}}}_{t}={{\hat{W}_{1}}}_{t}-{{\hat{Q}_{1}}}_{t}
\end{dmath}
% Equation 13
\begin{dmath}
{{\varphi}}\, {{\hat{L}_{2}}}_{t}+{{\sigma}}\, {{\hat{C}_{2}}}_{t}={{\hat{W}_{2}}}_{t}-{{\hat{Q}_{1}}}_{t}
\end{dmath}
% Equation 14
\begin{dmath}
{{\hat{Q}_{1}}}_{t+1}-{{\hat{Q}_{1}}}_{t}+{{\sigma}}\, \left({{\hat{C}_{1}}}_{t+1}-{{\hat{C}_{1}}}_{t}\right)=\left(1-{{\beta}}\right)\, {{\hat{R}}}_{t}
\end{dmath}
% Equation 15
\begin{dmath}
{{\hat{C}_{1}}}_{t+1}-{{\hat{C}_{1}}}_{t}={{\hat{C}_{2}}}_{t+1}-{{\hat{C}_{2}}}_{t}
\end{dmath}
% Equation 16
\begin{dmath}
{{\hat{Y}_{1}}}_{t}={{\hat{L}_{1}}}_{t}+{{\hat{Z}_{A1}}}_{t}
\end{dmath}
% Equation 17
\begin{dmath}
{{\hat{Y}_{2}}}_{t}={{\hat{L}_{2}}}_{t}+{{\hat{Z}_{A2}}}_{t}
\end{dmath}
% Equation 18
\begin{dmath}
{{\hat{\lambda}_{1}}}_{t}={{\hat{W}_{1}}}_{t}-{{\hat{Z}_{A1}}}_{t}-{{\hat{P}_{1}}}_{t}
\end{dmath}
% Equation 19
\begin{dmath}
{{\hat{\lambda}_{2}}}_{t}={{\hat{W}_{2}}}_{t}-{{\hat{Z}_{A2}}}_{t}-{{\hat{P}_{2}}}_{t}
\end{dmath}
% Equation 20
\begin{dmath}
{{\hat{R}}}_{t}={{\gamma_{R}}}\, {{\hat{R}}}_{t-1}+\left(1-{{\gamma_{R}}}\right)\, \left({{\gamma_{pi}}}\, {{\hat{\pi}}}_{t}+{{\gamma_{Y}}}\, {{\hat{Y}}}_{t}\right)+{{\hat{Z}_M}}_{t}
\end{dmath}
% Equation 21
\begin{dmath}
{{\hat{\pi}}}_{t}={{\hat{\pi}_{1}}}_{t}\, {thetapi}+{{\hat{\pi}_{2}}}_{t}\, \left(1-{thetapi}\right)
\end{dmath}
% Equation 22
\begin{dmath}
{{\hat{Y}}}_{t}={{\hat{Y}_{1}}}_{t}\, {thetaY}+{{\hat{Y}_{2}}}_{t}\, \left(1-{thetaY}\right)
\end{dmath}
% Equation 23
\begin{dmath}
{{\hat{P}_{1}}}_{t}+{{\hat{Y}_{1}}}_{t}={{\hat{C}_{1}}}_{t}+{{\hat{Q}_{1}}}_{t}
\end{dmath}
% Equation 24
\begin{dmath}
{{\hat{P}_{2}}}_{t}+{{\hat{Y}_{2}}}_{t}={{\hat{C}_{2}}}_{t}+{{\hat{Q}_{1}}}_{t}
\end{dmath}
% Equation 25
\begin{dmath}
{{\hat{Z}_{A1}}}_{t}={{\rho_{A1}}}\, {{\hat{Z}_{A1}}}_{t-1}+{{\varepsilon_{A1}}}_{t}
\end{dmath}
% Equation 26
\begin{dmath}
{{\hat{Z}_{A2}}}_{t}={{\rho_{A2}}}\, {{\hat{Z}_{A2}}}_{t-1}+{{\varepsilon_{A2}}}_{t}
\end{dmath}
% Equation 27
\begin{dmath}
{{\hat{Z}_M}}_{t}={{\rho_{M}}}\, {{\hat{Z}_M}}_{t-1}+{{\varepsilon_{M}}}_{t}
\end{dmath}
