\begin{dmath*}
Ps = 1
\end{dmath*}
\begin{dmath*}
PIs = 1
\end{dmath*}
\begin{dmath*}
ZAs = 1
\end{dmath*}
\begin{dmath*}
ZMs = 1
\end{dmath*}
\begin{dmath*}
Rs = {Ps}\, \left(\frac{1}{{{\beta}}}-\left(1-{{\delta}}\right)\right)
\end{dmath*}
\begin{dmath*}
LAMs = \frac{{Ps}\, \left({{\psi}}-1\right)}{{{\psi}}}
\end{dmath*}
\begin{dmath*}
Ws = \left(1-{{\alpha}}\right)\, \left({LAMs}\, {ZAs}\, \left(\frac{{{\alpha}}}{{Rs}}\right)^{{{\alpha}}}\right)^{\frac{1}{1-{{\alpha}}}}
\end{dmath*}
\begin{dmath*}
Ys = \left(\frac{{Ws}}{{Ps}\, {{\phi}}}\, \left(\frac{{Ws}}{\left(1-{{\alpha}}\right)\, {LAMs}}\right)^{{{\psi}}}\, \left(\frac{{Rs}}{{Rs}-{LAMs}\, {{\delta}}\, {{\alpha}}}\right)^{{{\sigma}}}\right)^{\frac{1}{{{\psi}}+{{\sigma}}}}
\end{dmath*}
\begin{dmath*}
Cs = \left(\frac{{Ws}}{{Ps}\, {{\phi}}}\, \left(\frac{{LAMs}\, \left(1-{{\alpha}}\right)\, {Ys}}{{Ws}}\right)^{\left(-{{\psi}}\right)}\right)^{\frac{1}{{{\sigma}}}}
\end{dmath*}
\begin{dmath*}
Ks = \frac{{LAMs}\, {{\alpha}}\, {Ys}}{{Rs}}
\end{dmath*}
\begin{dmath*}
Ls = \frac{{LAMs}\, \left(1-{{\alpha}}\right)\, {Ys}}{{Ws}}
\end{dmath*}
\begin{dmath*}
Is = {{\delta}}\, {Ks}
\end{dmath*}
\begin{dmath*}
RHO = \frac{1}{1+{Rs}}
\end{dmath*}
% Equation 1
\begin{dmath}
{{\tilde{\pi}}}_{t}={{\hat{P}}}_{t}-{{\hat{P}}}_{t-1}
\end{dmath}
% Equation 2
\begin{dmath}
{{\tilde{\pi}}}_{t}={RHO}\, {{\tilde{\pi}}}_{t+1}+\frac{{{\tilde{\lambda}}}_{t}\, \left(1-{{\theta}}\right)\, \left(1-{RHO}\, {{\theta}}\right)}{{{\theta}}}
\end{dmath}
% Equation 3
\begin{dmath}
{{\varphi}}\, {{\hat{L}}}_{t}+{{\sigma}}\, {{\hat{C}}}_{t}={{\hat{W}}}_{t}-{{\hat{P}}}_{t}
\end{dmath}
% Equation 4
\begin{dmath}
{{\hat{C}}}_{t+1}-{{\hat{C}}}_{t}=\frac{{Rs}\, {{\beta}}\, \left({{\hat{R}}}_{t+1}-{{\hat{P}}}_{t+1}\right)}{{Ps}\, {{\sigma}}}
\end{dmath}
% Equation 5
\begin{dmath}
{{\hat{K}}}_{t}=\left(1-{{\delta}}\right)\, {{\hat{K}}}_{t-1}+{{\delta}}\, {{\hat{I}}}_{t}
\end{dmath}
% Equation 6
\begin{dmath}
{{\tilde{\lambda}}}_{t}={{\alpha}}\, {{\hat{R}}}_{t}+\left(1-{{\alpha}}\right)\, {{\hat{W}}}_{t}-{{\hat{Z}^A}}_{t}-{{\hat{P}}}_{t}
\end{dmath}
% Equation 7
\begin{dmath}
{{\hat{Y}}}_{t}={{\hat{Z}^A}}_{t}+{{\alpha}}\, {{\hat{K}}}_{t-1}+\left(1-{{\alpha}}\right)\, {{\hat{L}}}_{t}
\end{dmath}
% Equation 8
\begin{dmath}
{{\hat{K}}}_{t-1}-{{\hat{L}}}_{t}={{\hat{W}}}_{t}-{{\hat{R}}}_{t}
\end{dmath}
% Equation 9
\begin{dmath}
{{\hat{Y}}}_{t}={{\hat{C}}}_{t}\, {{\theta_C}}+{{\hat{I}}}_{t}\, {{\theta_I}}
\end{dmath}
% Equation 10
\begin{dmath}
{{\hat{R}}}_{t}={{\gamma_R}}\, {{\hat{R}}}_{t-1}+\left(1-{{\gamma_R}}\right)\, \left({{\tilde{\pi}}}_{t}\, {{\gamma_\pi}}+{{\hat{Y}}}_{t}\, {{\gamma_Y}}\right)+{{\hat{Z}^M}}_{t}
\end{dmath}
% Equation 11
\begin{dmath}
{{\hat{Z}^A}}_{t}={{\rho_A}}\, {{\hat{Z}^A}}_{t-1}+{{\varepsilon_A}}_{t}
\end{dmath}
% Equation 12
\begin{dmath}
{{\hat{Z}^M}}_{t}={{\rho_M}}\, {{\hat{Z}^M}}_{t-1}+{{\varepsilon_M}}_{t}
\end{dmath}
